theories/quotlambda_new.v
@@ -1,0 +1,28 @@
+Require Import ssreflect ssrfun ssrbool ssrnat eqtype choice seq.
+Require Import bigop fintype finfun finset generic_quotient perm.
+Require Import tuple.
+Require Import fingroup.
+Require Import finmap.
+
+Set Implicit Arguments.
+Unset Strict Implicit.
+Unset Printing Implicit Defensive.
+
+Definition atom := nat.
+
+Record finPerm := FinPerm {
+  perm_of : {fmap atom -> atom};
+  _ : injectiveb (perm_of)
+}.
+
+Definition support (p : finPerm) :=
+  fset [seq a <- fset_keys (domf (perm_of p)) | fnd (perm_of p) a != Some a].
+
+Definition fun_of_perm (p:finPerm) (a:atom) :=
+  match fnd (perm_of p) a with
+      |Some x => x
+      |None => a
+  end.
+
+Coercion fun_of_perm : finPerm >-> Funclass.
+
